Ground_PDDL_Exec_Imp/Ground_PDDL_NTA_Reduction_Correctness.thy
@@ -34,6 +34,20 @@ begin
     shows "\<not>(\<exists>tp. valid_ground_plan P tp)"
     using valid_ground_plan_imp_form_holds assms by auto
 
+  lemma num_valid_ground_plan_imp_form_holds:
+    assumes "\<exists>\<pi>. abstr_model_checking.numeric_plan_for_problem \<pi>"
+    shows "abstr_model_checking.ref_model_checking.net_impl.sem,
+      abstr_model_checking.ref_model_checking.a\<^sub>0
+      \<Turnstile> abstr_model_checking.reduction_ref_impl.reach_formula"
+    using assms by (rule abstr_model_checking.numeric_valid_temp_plan_imp_form_holds)
+
+  corollary num_form_not_sat_imp_no_valid_ground_plan:
+    assumes "\<not>(abstr_model_checking.ref_model_checking.net_impl.sem,
+      abstr_model_checking.ref_model_checking.a\<^sub>0
+      \<Turnstile> abstr_model_checking.reduction_ref_impl.reach_formula)"
+    shows "\<not>(\<exists>\<pi>. abstr_model_checking.numeric_plan_for_problem \<pi>)"
+    using num_valid_ground_plan_imp_form_holds assms by auto
+
 end
 
 
